FTBFS monoid

examples/algebra/monoid/monoidOrderScript.sml
@@ -1079,24 +1079,24 @@ val lemma = prove(
    NOTE: added ‘(Monoid g /\ x NOTIN G* ==> y = ARB)’ to make it a total function.
  *)
 val lemma = prove(
-   “!(g:'a monoid) x. ?y. (Monoid g /\ x IN G* ==> y IN G /\ (x * y = #e) /\ (y * x = #e)) /\
-                          (Monoid g /\ x NOTIN G* ==> y = ARB)”,
+   “!(g:'a monoid) x.
+        ?y. (Monoid g /\ x IN G* ==> y IN G /\ (x * y = #e) /\ (y * x = #e)) /\
+            (Monoid g /\ x NOTIN G* ==> y = ARB)”,
     rpt GEN_TAC
  >> MP_TAC (Q.SPEC ‘g’ monoid_inv_from_invertibles)
  >> Cases_on ‘Monoid g’ >> rw []
  >> Cases_on ‘x IN G*’ >> rw []);
 
 (* Use Skolemization to generate the monoid_inv_from_invertibles function *)
-val extended_monoid_inv_def = new_specification(
-   "extended_monoid_inv_def",
-  ["monoid_inv"], (* name of function *)
+val ext_monoid_inv_def = new_specification(
+   "ext_monoid_inv_def", ["monoid_inv"], (* name of function *)
   SIMP_RULE (srw_ss()) [SKOLEM_THM] lemma);
 
 (* |- !g x. Monoid g /\ x IN G* ==>
             monoid_inv g x IN G /\ (x * monoid_inv g x = #e) /\
                                    (monoid_inv g x * x = #e)
  *)
-Theorem monoid_inv_def = cj 1 full_monoid_inv_def
+Theorem monoid_inv_def = cj 1 ext_monoid_inv_def
 (*
 - type_of ``monoid_inv g``;
 > val it = ``:'a -> 'a`` : hol_type
@@ -1224,5 +1224,6 @@ val monoid_invertibles_is_monoid = store_thm(
 
 (* export theory at end *)
 val _ = export_theory();
+val _ = html_theory "monoidOrder";
 
 (*===========================================================================*)
